WIP

src/example/LockClientSC.v
@@ -10,6 +10,8 @@ From Ordinal Require Export ClassicalHessenberg.
 
 Set Implicit Arguments.
 
+Definition ord_wf: WF := mk_wf (@Ord.lt_well_founded).
+
 Section INIT.
 
   Definition gvs : list nat := [1].
@@ -100,12 +102,15 @@ Section SIM.
   Context `{MONORA: @GRA.inG monoRA Σ}.
   Context `{THDRA: @GRA.inG ThreadRA Σ}.
   Context `{STATESRC: @GRA.inG (stateSrcRA (unit)) Σ}.
-  Context `{STATETGT: @GRA.inG (stateTgtRA (unit * SCMem.t * (bool * NatMap.t unit))) Σ}.
+  (* Context `{STATETGT: @GRA.inG (stateTgtRA (unit * (SCMem.t * (bool * NatMap.t unit)))) Σ}. *)
+  Context `{STATETGT: @GRA.inG (stateTgtRA ((OMod.closed_state ClientImpl.omod (ModAdd (SCMem.mod gvs) ABSLock.mod)))) Σ}.
   Context `{IDENTSRC: @GRA.inG (identSrcRA (void)) Σ}.
-  Context `{IDENTTGT: @GRA.inG (identTgtRA (void + SCMem.val + thread_id)%type) Σ}.
+  (* Context `{IDENTTGT: @GRA.inG (identTgtRA (void + (SCMem.val + thread_id))%type) Σ}. *)
+  Context `{IDENTTGT: @GRA.inG (identTgtRA (OMod.closed_ident ClientImpl.omod (ModAdd (SCMem.mod gvs) ABSLock.mod))%type) Σ}.
 
   Context `{OBLGRA: @GRA.inG ObligationRA.t Σ}.
-  Context `{ARROWRA: @GRA.inG (ArrowRA (void + SCMem.val + thread_id)%type) Σ}.
+  (* Context `{ARROWRA: @GRA.inG (ArrowRA (void + (SCMem.val + thread_id))%type) Σ}. *)
+  Context `{ARROWRA: @GRA.inG (ArrowRA (OMod.closed_ident ClientImpl.omod (ModAdd (SCMem.mod gvs) ABSLock.mod))%type) Σ}.
   Context `{EDGERA: @GRA.inG EdgeRA Σ}.
   Context `{ONESHOTSRA: @GRA.inG (@FiniteMap.t (OneShot.t unit)) Σ}.
 
@@ -131,21 +136,21 @@ Section SIM.
             ∨
               (ObligationRA.shot k ∗ points_to loc_X const_42)).
 
-  Definition lock_will_unlock (own: bool) (ths wait: TIdSet.t) : iProp :=
-    ∃ (f: NatMap.t nat) (j: nat),
+  Definition lock_will_unlock (own: bool) (wait: TIdSet.t) : iProp :=
+    ∃ (ths: TIdSet.t) (f: NatMap.t nat) (j: nat),
       (OwnM (Auth.black (Some f: NatMapRA.t nat)))
         ∗
         (OwnM (Auth.black (Excl.just j: Excl.t nat)))
         ∗
         (⌜nm_wf_pair f wait⌝)
         ∗
-        (natmap_prop_sum ths (fun tid _ => (⌜~ NatMap.In tid wait⌝) -∗ ObligationRA.duty (inr (inr tid)) []))
+        (natmap_prop_sum ths (fun tid _ => (⌜~ NatMap.In tid wait⌝) -∗ ObligationRA.duty (inr (inr (inr tid))) []))
         ∗
-        (natmap_prop_sum f (fun tid idx => (ObligationRA.correl (inr (inr tid)) idx (Ord.omega ^ 2)%ord)
+        (natmap_prop_sum f (fun tid idx => (ObligationRA.correl (inr (inr (inr tid))) idx (Ord.omega ^ 2)%ord)
                                           ∗
                                           (ObligationRA.pending idx 1)
                                           ∗
-                                          (ObligationRA.duty (inr (inr tid)) [(idx, Ord.omega)])
+                                          (ObligationRA.duty (inr (inr (inr tid))) [(idx, Ord.omega)])
         ))
         ∗
         ((⌜own = false⌝ ∗ OwnM (Auth.white (Excl.just j: Excl.t nat)))
@@ -158,30 +163,34 @@ Section SIM.
         )
   .
 
-  Definition lock_holding (j: nat) (n: Ord.t) : iProp :=
-    (OwnM (Auth.black (Excl.just j: Excl.t nat))) ∗ (ObligationRA.white j n).
+  Definition lock_holding: iProp :=
+    ∃ (j: nat) (n: Ord.t),
+      (OwnM (Auth.black (Excl.just j: Excl.t nat))) ∗ (ObligationRA.white j n).
 
-  Definition lock_waiting (tid: thread_id) (i: nat) : iProp :=
-    ∃ m, (OwnM (Auth.white (NatMapRA.singleton tid i: NatMapRA.t nat)))
-           ∗
-           (ObligationRA.correl (inr (inr tid)) i (Ord.omega ^ 2)%ord)
-           ∗
-           (ObligationRA.black i m).
+  Definition lock_waiting: iProp :=
+    ∃ (tid: thread_id) (i: nat) m,
+      (OwnM (Auth.white (NatMapRA.singleton tid i: NatMapRA.t nat)))
+        ∗
+        (ObligationRA.correl (inr (inr (inr tid))) i (Ord.omega ^ 2)%ord)
+        ∗
+        (ObligationRA.black i m).
 
-  Let config := [("thread1", tt↑); ("thread2", tt↑)].
+  Let I: list iProp :=
+        [thread1_will_write; lock_will_unlock false TIdSet.empty; lock_holding; lock_waiting].
 
-  Lemma client_correct:
-    UserSim.sim ClientSpec.mod ClientImpl.mod
-                (prog2ths ClientSpec.mod config)
-                (prog2ths ClientImpl.mod config).
+  Lemma correct_thread1:
+    (own_thread 0 ∗ ObligationRA.duty (inl 0) []) ⊢
+          (stsim I 0 [0; 1; 2; 3] ibot5 ibot5
+                (fun r_src r_tgt => own_thread 0 ** ObligationRA.duty (inl 1) [] ** ⌜r_src = r_tgt⌝)
+                (ClientSpec.thread1 tt)
+                (OMod.close_itree ClientImpl.omod (ModAdd (SCMem.mod gvs) ABSLock.mod) (ClientImpl.thread1 tt))).
   Proof.
-    refine (@ModSim.mk _ _ nat_wf nat_wf _ _ Σ _ _ _).
-    { econs. exact 0. }
-    { i. exists (S o0). ss. }
-    { admit. }
-    { cut (forall tid,
-              (own_thread tid ** ObligationRA.duty (inl tid) []) ⊢ stsim I tid [0; 1] ibot5 ibot5 (fun r_src r_tgt => own_thread tid ** ObligationRA.duty (inl tid) [] ** ⌜r_src = r_tgt⌝) (example_spec_fun tt) (OMod.close_itree (example_omod) (SCMem.mod [1; 1]) (example_fun tt))).
-      { admit. }
+    iIntros "[TH DUTY]". 
+
+
+
+
+    
       iIntros (?) "[TH DUTY]". unfold example_spec_fun, example_fun.
       lred. rred. rewrite close_itree_call. ss. rred.
       iApply (stsim_yieldR with "[DUTY]"); [msubtac|iFrame|]. iIntros "DUTY _".
@@ -192,6 +201,234 @@ Section SIM.
       rred. iApply stsim_tauR. rred.
       unfold SCMem.cas.
       iopen 1 "[[[POINTL POINTF] PEND]|[% H]]" "K1".
+      { iPoseProof (memory_ra_load with "MEM POINTL") as "%". des; clarify.
+        rewrite H. ss.
+        iPoseProof (memory_ra_store with "MEM POINTL") as "[% [% > [MEM POINTL]]]".
+        rewrite H1. ss.
+        rred. iApply stsim_getR. iSplit.
+        { iFrame. }
+        rred. iApply (stsim_putR with "ST"). iIntros "ST".
+        rred. iApply stsim_tauR.
+        rred. iApply stsim_tauR.
+        rred.
+        iPoseProof (@ObligationRA.alloc _ _ ((1 × Ord.omega) × 10)%ord) as "> [% [[# BLACK WHITES] OBL]]".
+        iPoseProof (ObligationRA.cut_white with "WHITES") as "[WHITES WHITE]".
+        iPoseProof (ObligationRA.duty_alloc with "DUTY WHITE") as "> DUTY".
+        iPoseProof (ObligationRA.duty_correl_thread with "DUTY") as "# CORR"; [ss; eauto|].
+        iPoseProof (OwnM_Upd with "PEND") as "> SHOT".
+        { eapply (OneShot.pending_shot k). }
+        iPoseProof (own_persistent with "SHOT") as "# SHOTP". iClear "SHOT". ss.
+        iMod ("K0" with "[MEM ST]") as "_".
+        { iExists _. iFrame. }
+        iPoseProof (ObligationRA.pending_split with "[OBL]") as "[OBL0 OBL1]".
+        { rewrite Qp_inv_half_half. iFrame. }
+        iMod ("K1" with "[POINTF POINTL OBL1]") as "_".
+        { iRight. iExists _. iFrame. iSplitR.
+          { iSplit; [iSplit; [iApply "SHOTP"|iApply "CORR"]|eauto]. }
+          { iLeft. iFrame. }
+        }
+        { msubtac. }
+        iPoseProof (ObligationRA.cut_white with "WHITES") as "[WHITES WHITE]".
+        msimpl. iApply (stsim_yieldR with "[DUTY WHITE]").
+        { msubtac. }
+        { iFrame. iSplit; auto. }
+        iIntros "DUTY _".
+        rred. iApply stsim_tauR.
+        iPoseProof (ObligationRA.cut_white with "WHITES") as "[WHITES WHITE]".
+        rred. iApply (stsim_yieldR with "[DUTY WHITE]").
+        { msubtac. }
+        { iFrame. iSplit; auto. }
+        iIntros "DUTY _".
+        rred. iApply stsim_tauR.
+        rred. rewrite close_itree_call. ss.
+        iPoseProof (ObligationRA.cut_white with "WHITES") as "[WHITES WHITE]".
+        rred. iApply (stsim_yieldR with "[DUTY WHITE]").
+        { msubtac. }
+        { iFrame. iSplit; auto. }
+        iIntros "DUTY _".
+        unfold SCMem.store_fun, Mod.wrap_fun. rred.
+        iopen 0 "[% [MEM ST]]" "K0".
+        iApply stsim_getR. iSplit.
+        { iFrame. }
+        rred. iApply stsim_tauR. rred.
+        iopen 1 "[[[POINTL POINTF] PEND]|[% [H H1]]]" "K1".
+        { iExFalso. iApply OneShotP.pending_not_shot. iSplit; iFrame. auto. }
+        { iPoseProof (OneShotP.shot_agree with "[H]") as "%".
+          { iSplit.
+            { iApply "SHOTP". }
+            { iDestruct "H" as "[[[H _] _] _]". iApply "H". }
+          }
+          subst.
+          iDestruct "H1" as "[[POINTF PEND]|[POINTF OBL1]]".
+          { iPoseProof (memory_ra_store with "MEM POINTF") as "[% [% > [MEM POINTF]]]".
+            rewrite H2. ss.
+            rred. iApply stsim_getR. iSplit.
+            { iFrame. }
+            rred. iApply (stsim_putR with "ST"). iIntros "ST".
+            rred. iApply stsim_tauR.
+            rred. iApply stsim_tauR. rred.
+            iMod ("K0" with "[MEM ST]") as "_".
+            { iExists _. iFrame. }
+            iPoseProof (ObligationRA.pending_shot with "[OBL0 PEND]") as "> # OSHOT".
+            { rewrite <- Qp_inv_half_half. iApply (ObligationRA.pending_sum with "OBL0 PEND"). }
+            iMod ("K1" with "[POINTF H OSHOT]") as "_".
+            { iRight. iExists _. iFrame. iRight. iFrame. auto. }
+            { msubtac. }
+            iPoseProof (ObligationRA.duty_done with "DUTY OSHOT") as "> DUTY".
+            iApply (stsim_sync with "[DUTY]").
+            { msubtac. }
+            { iFrame. }
+            iIntros "DUTY _".
+            iApply stsim_tauR.
+            iApply stsim_ret. iModIntro. iFrame. auto.
+          }
+          { iExFalso. iApply (ObligationRA.pending_not_shot with "OBL0 OBL1"). }
+        }
+      }
+      { iDestruct "H" as "[[[[# SHOTK # CORR] [% # BLACK]] POINTL] F]".
+        iPoseProof (memory_ra_load with "MEM POINTL") as "%". des; clarify.
+        rewrite H. ss.
+        rred. iApply stsim_tauR.
+        iMod ("K0" with "[MEM ST]") as "_".
+        { iExists _. iFrame. }
+        iMod ("K1" with "[POINTL F]") as "_".
+        { iRight. iExists _. iFrame. auto. }
+        { msubtac. }
+        rred. iStopProof. pattern n. revert n.
+        apply (well_founded_induction Ord.lt_well_founded). intros o IH.
+        iIntros "[# [SHOTK [CORR BLACK]] [TH DUTY]]".
+        rewrite OpenMod.unfold_iter. rred.
+        iApply (stsim_yieldR with "[DUTY]").
+        { msubtac. }
+        { iFrame. }
+        iIntros "DUTY WHITE".
+        rred. iApply stsim_tauR. rred.
+        rewrite close_itree_call. ss.
+        unfold SCMem.load_fun, Mod.wrap_fun.
+        rred. iApply (stsim_yieldR with "[DUTY]").
+        { msubtac. }
+        { iFrame. }
+        iIntros "DUTY _".
+        iopen 0 "[% [MEM ST]]" "K0".
+        rred. iApply stsim_getR. iSplit.
+        { iFrame. }
+        rred. iApply stsim_tauR. rred.
+        iopen 1 "[FALSE|[% H]]" "K1".
+        { iExFalso. iApply OneShotP.pending_not_shot. iSplit; [|iApply "SHOTK"].
+          iDestruct "FALSE" as "[[? ?] ?]". iFrame.
+        }
+        iDestruct "H" as "[X [Y|Y]]".
+        { iPoseProof (OneShotP.shot_agree with "[X]") as "%".
+          { iSplit.
+            { iApply "SHOTK". }
+            { iDestruct "X" as "[[[H ?] ?] ?]". iApply "H". }
+          }
+          subst.
+          iPoseProof (ObligationRA.correl_thread_correlate with "CORR WHITE") as "> [WHITE|WHITE]"; cycle 1.
+          { iExFalso. iApply (ObligationRA.pending_not_shot with "[Y] WHITE").
+            iDestruct "Y" as "[_ ?]". eauto.
+          }
+          iPoseProof (memory_ra_load with "MEM [Y]") as "%".
+          { iDestruct "Y" as "[? _]". iFrame. }
+          des. rewrite H1.
+          rred. iApply stsim_tauR.
+          iMod ("K0" with "[MEM ST]") as "_".
+          { iExists _. iFrame. }
+          iMod ("K1" with "[X Y]") as "_".
+          { iRight. iExists _. iFrame. }
+          { msubtac. }
+          rred. iApply (stsim_yieldR with "[DUTY]").
+          { msubtac. }
+          { iFrame. }
+          iIntros "DUTY _".
+          rred. iApply stsim_tauR.
+          rred. rewrite close_itree_call. ss.
+          unfold SCMem.compare_fun, Mod.wrap_fun.
+          rred. iApply (stsim_yieldR with "[DUTY]").
+          { msubtac. }
+          { iFrame. }
+          iIntros "DUTY _".
+          iopen 0 "[% [MEM ST]]" "K0".
+          rred. iApply stsim_getR. iSplit.
+          { iFrame. }
+          iMod ("K0" with "[MEM ST]") as "_".
+          { iExists _. iFrame. }
+          { msubtac. }
+          rred. iApply stsim_tauR.
+          rred. iApply stsim_tauR.
+          rred. iApply (stsim_yieldR with "[DUTY]").
+          { msubtac. }
+          { iFrame. }
+          iIntros "DUTY _".
+          rred. iApply stsim_tauR.
+          rred. iApply stsim_tauR.
+          iPoseProof (ObligationRA.black_white_decr_one with "BLACK WHITE") as "> [% [# BLACK1 %]]".
+          iApply IH; eauto. iFrame. iModIntro. iSplit; auto.
+        }
+        { iPoseProof (memory_ra_load with "MEM [Y]") as "%".
+          { iDestruct "Y" as "[? _]". iFrame. }
+          des. rewrite H1.
+          rred. iApply stsim_tauR.
+          iMod ("K0" with "[MEM ST]") as "_".
+          { iExists _. iFrame. }
+          iMod ("K1" with "[X Y]") as "_".
+          { iRight. iExists _. iFrame. }
+          { msubtac. }
+          rred. iApply (stsim_yieldR with "[DUTY]").
+          { msubtac. }
+          { iFrame. }
+          iIntros "DUTY _".
+          rred. iApply stsim_tauR.
+          rred. rewrite close_itree_call. ss.
+          unfold SCMem.compare_fun, Mod.wrap_fun.
+          rred. iApply (stsim_yieldR with "[DUTY]").
+          { msubtac. }
+          { iFrame. }
+          iIntros "DUTY _".
+          iopen 0 "[% [MEM ST]]" "K0".
+          rred. iApply stsim_getR. iSplit.
+          { iFrame. }
+          iMod ("K0" with "[MEM ST]") as "_".
+          { iExists _. iFrame. }
+          { msubtac. }
+          rred. iApply stsim_tauR.
+          rred. iApply stsim_tauR.
+          rred. iApply (stsim_sync with "[DUTY]").
+          { msubtac. }
+          { iFrame. }
+          iIntros "DUTY _".
+          rred. iApply stsim_tauR.
+          rred. iApply stsim_ret.
+          iModIntro. iFrame. auto.
+        }
+      }
+
+  Abort.
+
+  Let config := [("thread1", tt↑); ("thread2", tt↑)].
+
+  Lemma client_correct:
+    UserSim.sim ClientSpec.mod ClientImpl.mod
+                (prog2ths ClientSpec.mod config)
+                (prog2ths ClientImpl.mod config).
+  Proof.
+    refine (@UserSim.mk _ _ _ _ ord_wf nat_wf _ _ Σ _ _).
+    { econs. exact 0. }
+    { i. exists (S o0). ss. }
+    ss.
+    cut (forall tid,
+            (own_thread tid ** ObligationRA.duty (inl tid) []) ⊢ stsim I tid [0; 1] ibot5 ibot5 (fun r_src r_tgt => own_thread tid ** ObligationRA.duty (inl tid) [] ** ⌜r_src = r_tgt⌝) (example_spec_fun tt) (OMod.close_itree (example_omod) (SCMem.mod [1; 1]) (example_fun tt))).
+    { admit. }
+    iIntros (?) "[TH DUTY]". unfold example_spec_fun, example_fun.
+    lred. rred. rewrite close_itree_call. ss. rred.
+    iApply (stsim_yieldR with "[DUTY]"); [msubtac|iFrame|]. iIntros "DUTY _".
+    rred. unfold SCMem.cas_fun, Mod.wrap_fun. rred.
+    iopen 0 "[% [MEM ST]]" "K0".
+    iApply stsim_getR. iSplit.
+    { iFrame. }
+    rred. iApply stsim_tauR. rred.
+    unfold SCMem.cas.
+    iopen 1 "[[[POINTL POINTF] PEND]|[% H]]" "K1".
   Abort.
 
 End SIM.
